renamed inv6

src/proofs/no_slashable_attestations/supporting_lemmas/inv.dfy
@@ -1424,18 +1424,18 @@ module Att_Inv_With_Empty_Initial_Attestation_Slashing_DB
             && inv5_body(dvc)
     }
 
-    predicate inv6_body(dvc: DVCState)
+    predicate inv_current_att_duty_is_rcvd_duty_body(dvc: DVCState)
     {
         dvc.current_attestation_duty.isPresent()
             ==> dvc.current_attestation_duty.safe_get()
                     in dvc.all_rcvd_duties
     }
 
-    predicate inv6(dv: DVState)
+    predicate inv_current_att_duty_is_rcvd_duty(dv: DVState)
     {
         forall hn: BLSPubkey | hn in dv.honest_nodes_states.Keys ::            
             && var dvc := dv.honest_nodes_states[hn];
-            && inv6_body(dvc)
+            && inv_current_att_duty_is_rcvd_duty_body(dvc)
     }
 
     predicate inv_latest_served_duty_is_rcvd_duty_body(dvc: DVCState)
